feat: Semantics

Logic/Predicate/FirstOrder/Semantics.lean
@@ -1,5 +1,6 @@
 import Logic.Predicate.FirstOrder.Calculus
 import Logic.Predicate.Semantics
+import Logic.Vorspiel.Logic
 
 universe u u₁ u₂ v v₁ v₂ w w₁ w₂
 
@@ -11,90 +12,90 @@ namespace SubFormula
 variable {n : ℕ} {M : Type w} (s : Structure₁ L M)
   (e : Fin n → M) (e₂ : Fin n₂ → M) (ε : μ → M) (ε₂ : μ₂ → M)
 
-def SubVal' (ε : μ → M) : ∀ {n}, (Fin n → M) → SubFormula L μ n → Prop
+def Eval' (ε : μ → M) : ∀ {n}, (Fin n → M) → SubFormula L μ n → Prop
   | _, _, ⊤        => True
   | _, _, ⊥        => False
   | _, e, rel p v  => Structure₁.rel p (fun i => SubTerm.val s e ε (v i))
   | _, e, nrel p v => ¬Structure₁.rel p (fun i => SubTerm.val s e ε (v i))
-  | _, e, p ⋏ q    => p.SubVal' ε e ∧ q.SubVal' ε e
-  | _, e, p ⋎ q    => p.SubVal' ε e ∨ q.SubVal' ε e
-  | _, e, ∀' p     => ∀ x : M, (p.SubVal' ε (x :> e))
-  | _, e, ∃' p     => ∃ x : M, (p.SubVal' ε (x :> e))
+  | _, e, p ⋏ q    => p.Eval' ε e ∧ q.Eval' ε e
+  | _, e, p ⋎ q    => p.Eval' ε e ∨ q.Eval' ε e
+  | _, e, ∀' p     => ∀ x : M, (p.Eval' ε (x :> e))
+  | _, e, ∃' p     => ∃ x : M, (p.Eval' ε (x :> e))
 
-@[simp] lemma SubVal'_neg (p : SubFormula L μ n) :
-    SubVal' s ε e (~p) = ¬SubVal' s ε e p :=
-  by induction p using rec' <;> simp[*, SubVal', ←neg_eq, or_iff_not_imp_left]
+@[simp] lemma Eval'_neg (p : SubFormula L μ n) :
+    Eval' s ε e (~p) = ¬Eval' s ε e p :=
+  by induction p using rec' <;> simp[*, Eval', ←neg_eq, or_iff_not_imp_left]
 
-def SubVal : SubFormula L μ n →L Prop where
-  toFun := SubVal' s ε e
+def Eval : SubFormula L μ n →L Prop where
+  toFun := Eval' s ε e
   map_top' := rfl
   map_bot' := rfl
-  map_and' := by simp[SubVal']
-  map_or' := by simp[SubVal']
-  map_neg' := by simp[SubVal'_neg]
-  map_imp' := by simp[imp_eq, SubVal'_neg, ←neg_eq, SubVal', imp_iff_not_or]
+  map_and' := by simp[Eval']
+  map_or' := by simp[Eval']
+  map_neg' := by simp[Eval'_neg]
+  map_imp' := by simp[imp_eq, Eval'_neg, ←neg_eq, Eval', imp_iff_not_or]
 
-abbrev SubVal! (M : Type w) [s : Structure₁ L M] {n} (e : Fin n → M) (ε : μ → M) :
-    SubFormula L μ n →L Prop := SubVal s e ε
+abbrev Eval! (M : Type w) [s : Structure₁ L M] {n} (e : Fin n → M) (ε : μ → M) :
+    SubFormula L μ n →L Prop := Eval s e ε
 
-abbrev Val (ε : μ → M) : Formula L μ →L Prop := SubVal s ![] ε
+abbrev Realize (ε : μ → M) : Formula L μ →L Prop := Eval s ![] ε
 
-abbrev Val! (M : Type w) [s : Structure₁ L M] (ε : μ → M) :
-    Formula L μ →L Prop := Val s ε
+abbrev Realize! (M : Type w) [s : Structure₁ L M] (ε : μ → M) :
+    Formula L μ →L Prop := Realize s ε
 
-lemma subVal_rel {k} {r : L.rel k} {v} :
-    SubVal s e ε (rel r v) ↔ s.rel r (fun i => SubTerm.val s e ε (v i)) := of_eq rfl
+lemma eval_rel {k} {r : L.rel k} {v} :
+    Eval s e ε (rel r v) ↔ s.rel r (fun i => SubTerm.val s e ε (v i)) := of_eq rfl
 
-@[simp] lemma subVal_rel₀ {r : L.rel 0} :
-    SubVal s e ε (rel r ![]) ↔ s.rel r ![] := by simp[subVal_rel, Matrix.empty_eq]
+@[simp] lemma eval_rel₀ {r : L.rel 0} :
+    Eval s e ε (rel r ![]) ↔ s.rel r ![] := by simp[eval_rel, Matrix.empty_eq]
 
-@[simp] lemma subVal_rel₁ {r : L.rel 1} (t : SubTerm L μ n) :
-    SubVal s e ε (rel r ![t]) ↔ s.rel r ![t.val s e ε] := by
-  simp[subVal_rel]; apply of_eq; congr
+@[simp] lemma eval_rel₁ {r : L.rel 1} (t : SubTerm L μ n) :
+    Eval s e ε (rel r ![t]) ↔ s.rel r ![t.val s e ε] := by
+  simp[eval_rel]; apply of_eq; congr
   funext i; cases' i using Fin.cases with i <;> simp
 
-@[simp] lemma subVal_rel₂ {r : L.rel 2} (t₁ t₂ : SubTerm L μ n) :
-    SubVal s e ε (rel r ![t₁, t₂]) ↔ s.rel r ![t₁.val s e ε, t₂.val s e ε] := by
-  simp[subVal_rel]; apply of_eq; congr
+@[simp] lemma eval_rel₂ {r : L.rel 2} (t₁ t₂ : SubTerm L μ n) :
+    Eval s e ε (rel r ![t₁, t₂]) ↔ s.rel r ![t₁.val s e ε, t₂.val s e ε] := by
+  simp[eval_rel]; apply of_eq; congr
   funext i; cases' i using Fin.cases with i <;> simp
 
-lemma subVal_nrel {k} {r : L.rel k} {v} :
-    SubVal s e ε (nrel r v) ↔ ¬s.rel r (fun i => SubTerm.val s e ε (v i)) := of_eq rfl
+lemma eval_nrel {k} {r : L.rel k} {v} :
+    Eval s e ε (nrel r v) ↔ ¬s.rel r (fun i => SubTerm.val s e ε (v i)) := of_eq rfl
 
-@[simp] lemma subVal_nrel₀ {r : L.rel 0} :
-    SubVal s e ε (nrel r ![]) ↔ ¬s.rel r ![] := by simp[subVal_nrel, Matrix.empty_eq]
+@[simp] lemma eval_nrel₀ {r : L.rel 0} :
+    Eval s e ε (nrel r ![]) ↔ ¬s.rel r ![] := by simp[eval_nrel, Matrix.empty_eq]
 
-@[simp] lemma subVal_nrel₁ {r : L.rel 1} (t : SubTerm L μ n) :
-    SubVal s e ε (nrel r ![t]) ↔ ¬s.rel r ![t.val s e ε] := by
-  simp[subVal_rel]; apply of_eq; congr
+@[simp] lemma eval_nrel₁ {r : L.rel 1} (t : SubTerm L μ n) :
+    Eval s e ε (nrel r ![t]) ↔ ¬s.rel r ![t.val s e ε] := by
+  simp[eval_rel]; apply of_eq; congr
   funext i; cases' i using Fin.cases with i <;> simp
 
-@[simp] lemma subVal_nrel₂ {r : L.rel 2} (t₁ t₂ : SubTerm L μ n) :
-    SubVal s e ε (nrel r ![t₁, t₂]) ↔ ¬s.rel r ![t₁.val s e ε, t₂.val s e ε] := by
-  simp[subVal_rel]; apply of_eq; congr
+@[simp] lemma eval_nrel₂ {r : L.rel 2} (t₁ t₂ : SubTerm L μ n) :
+    Eval s e ε (nrel r ![t₁, t₂]) ↔ ¬s.rel r ![t₁.val s e ε, t₂.val s e ε] := by
+  simp[eval_rel]; apply of_eq; congr
   funext i; cases' i using Fin.cases with i <;> simp
 
-@[simp] lemma subVal_all {p : SubFormula L μ (n + 1)} :
-    SubVal s e ε (∀' p) ↔ ∀ x : M, SubVal s (x :> e) ε p := of_eq rfl
+@[simp] lemma eval_all {p : SubFormula L μ (n + 1)} :
+    Eval s e ε (∀' p) ↔ ∀ x : M, Eval s (x :> e) ε p := of_eq rfl
 
-@[simp] lemma subVal_ex {p : SubFormula L μ (n + 1)} :
-    SubVal s e ε (∃' p) ↔ ∃ x : M, SubVal s (x :> e) ε p := of_eq rfl
+@[simp] lemma eval_ex {p : SubFormula L μ (n + 1)} :
+    Eval s e ε (∃' p) ↔ ∃ x : M, Eval s (x :> e) ε p := of_eq rfl
 
-lemma subVal_bind (bound : Fin n₁ → SubTerm L μ₂ n₂) (free : μ₁ → SubTerm L μ₂ n₂) (p : SubFormula L μ₁ n₁) :
-    SubVal s e₂ ε₂ (bind bound free p) =
-    SubVal s (SubTerm.val s e₂ ε₂ ∘ bound) (SubTerm.val s e₂ ε₂ ∘ free) p := by
+lemma eval_bind (bound : Fin n₁ → SubTerm L μ₂ n₂) (free : μ₁ → SubTerm L μ₂ n₂) (p : SubFormula L μ₁ n₁) :
+    Eval s e₂ ε₂ (bind bound free p) =
+    Eval s (SubTerm.val s e₂ ε₂ ∘ bound) (SubTerm.val s e₂ ε₂ ∘ free) p := by
   induction p using rec' generalizing n₂ <;> simp[*, SubTerm.val_bind, Function.comp,
-    bind_rel, bind_nrel, subVal_rel, subVal_nrel]
+    bind_rel, bind_nrel, eval_rel, eval_nrel]
   · apply forall_congr'; intros a; apply of_eq; congr; exact funext $ Fin.cases (by simp) (by simp)
   · apply exists_congr; intros a; apply of_eq; congr; exact funext $ Fin.cases (by simp) (by simp)
 
-lemma subVal_map (bound : Fin n₁ → Fin n₂) (free : μ₁ → μ₂) (e : Fin n₂ → M) (ε : μ₂ → M) (p : SubFormula L μ₁ n₁) :
-    SubVal s e ε (map bound free p) = SubVal s (e ∘ bound) (ε ∘ free) p :=
-  by simp[map, subVal_bind, Function.comp]
+lemma eval_map (bound : Fin n₁ → Fin n₂) (free : μ₁ → μ₂) (e : Fin n₂ → M) (ε : μ₂ → M) (p : SubFormula L μ₁ n₁) :
+    Eval s e ε (map bound free p) = Eval s (e ∘ bound) (ε ∘ free) p :=
+  by simp[map, eval_bind, Function.comp]
 
-lemma subVal_subst (u : SubTerm L μ n) (p : SubFormula L μ (n + 1)) :
-    SubVal s e ε (subst u p) = SubVal s (e <: u.val s e ε) ε p :=
-  by simp[subst, subVal_bind]; apply of_eq; congr ; exact funext $ Fin.lastCases (by simp) (by simp)
+lemma eval_subst (u : SubTerm L μ n) (p : SubFormula L μ (n + 1)) :
+    Eval s e ε (subst u p) = Eval s (e <: u.val s e ε) ε p :=
+  by simp[subst, eval_bind]; apply of_eq; congr ; exact funext $ Fin.lastCases (by simp) (by simp)
 
 section Syntactic
 variable (Ψ : ℕ → M)
@@ -103,74 +104,65 @@ end Syntactic
 
 end SubFormula
 
-notation:50 M " ⊧₁[" e :80 "] "p :0 => SubFormula.Val! M e p
+def Models {M : Type w} (s : Structure₁ L M)  : Sentence L →L Prop := SubFormula.Realize s Empty.elim
 
-def Models (s : Structure₁ L M) (p : Formula L μ) : Prop := ∀ ε, SubFormula.Val s ε p
+instance : Semantics.{u, u, u} (Sentence L) where
+  struc := Structure₁ L
+  models := Models
 
-instance : HasDoubleTurnstile (Structure₁ L M) (Formula L μ) := ⟨Models⟩
+@[reducible] instance toCStruc [s : Structure₁ L M] : Semantics.CStruc (Sentence L) M := ⟨s⟩
 
-@[reducible] def models! (M : Type w) [s : Structure₁ L M] (p : Formula L μ) : Prop := s ⊧ p
+abbrev toStruc (s : Structure₁ L M) : Semantics.struc (Sentence L) M := s
 
-infix:50 " ⊧₁ " => models!
+section
+variable {M : Type u} {s : Structure₁ L M}
 
-def ModelsTheory (s : Structure₁ L M) (T : Theory L μ) : Prop := ∀ p ∈ T, s ⊧ p
+lemma models_def : M ⊧ = SubFormula.Realize s Empty.elim := rfl
 
-instance : HasDoubleTurnstile (Structure₁ L M) (Theory L μ) := ⟨ModelsTheory⟩
+lemma modelsₛ_def : (toStruc s) ⊧ₛ = SubFormula.Realize s Empty.elim := rfl
 
-lemma models_def {s : Structure₁ L M} {p : Formula L μ} : s ⊧ p ↔ (∀ e, SubFormula.Val s e p) :=
-  by simp[HasDoubleTurnstile.doubleTurnstile, Models]
+lemma models_iff {σ : Sentence L} : M ⊧ σ ↔ SubFormula.Realize s Empty.elim σ := by simp[models_def]
 
-lemma models_sentence_def {s : Structure₁ L M} {σ : Sentence L} : s ⊧ σ ↔ SubFormula.Val s Empty.elim σ :=
-  by simp[HasDoubleTurnstile.doubleTurnstile, Models, Empty.eq_elim]
+lemma models_iff_modelsₛ {σ : Sentence L} : M ⊧ σ ↔ (toStruc s) ⊧ₛ σ := by simp[models_def, modelsₛ_def]
 
-def Valid (p : Formula L μ) : Prop := ∀ {M : Type u} [Inhabited M] (s : Structure₁ L M), s ⊧ p
+lemma modelsTheory_def {T : CTheory L} : M ⊧* T ↔ (∀ ⦃σ⦄, σ ∈ T → M ⊧ σ) :=
+  by simp[Semantics.cmodelsTheory]
 
-instance : HasDoubleTurnstile (Theory L μ) (Formula L μ) :=
-  ⟨fun T p => ∀ {M : Type u} [Inhabited M] (s : Structure₁ L M), (∀ q ∈ T, s ⊧ q) → s ⊧ p⟩
+lemma modelsₛ_iff {σ : Sentence L} :
+  (toStruc s) ⊧ₛ σ ↔ SubFormula.Realize s Empty.elim σ := of_eq rfl
 
-lemma semanticConsequence_def {T : Theory L μ} {p : Formula L μ} :
-    T ⊧ p ↔ (∀ {M : Type u} [Inhabited M] (s : Structure₁ L M), (∀ q ∈ T, s ⊧ q) → s ⊧ p) :=
-  by simp[HasDoubleTurnstile.doubleTurnstile, Models]
+lemma consequence_iff {T : CTheory L} {σ : Sentence L} :
+    T ⊨ σ ↔ (∀ (M : Type u) [Inhabited M] (_ : Structure₁ L M), M ⊧* T → M ⊧ σ) :=
+  Semantics.consequence_iff
 
-lemma semanticConsequence_def! {T : Theory L μ} {p : Formula L μ} :
-    T ⊧ p ↔ (∀ (M : Type u) [Inhabited M] [Structure₁ L M], (∀ q ∈ T, M ⊧₁ q) → M ⊧₁ p) :=
-  by simp[semanticConsequence_def]
+lemma satisfiableₛ_iff {T : CTheory L} :
+    Semantics.Satisfiableₛ T ↔ ∃ (M : Type u) (_ : Inhabited M) (_ : Structure₁ L M), M ⊧* T :=
+  Semantics.satisfiableₛ_iff
 
-lemma valid_def! {p : Formula L μ} :
-    Valid p ↔ ∀ (M : Type u) [Inhabited M] [Structure₁ L M], M ⊧₁ p := of_eq rfl
-
-@[simp] lemma Valid_top : Valid (⊤ : Formula L μ) := by simp[Valid, models_def]; simp[Top.top]
-
-@[simp] lemma nValid_bot : ¬Valid (⊥ : Formula L μ) := by
-  simp[Valid]
-  exact ⟨PUnit, instInhabitedPUnit, default, by simp[models_def]; simp[Bot.bot]⟩
-
-def SubFormula.Satisfiable (p : Formula L μ) : Prop :=
-  ∃ (M : Type u) (_ : Inhabited M) (s : Structure₁ L M), s ⊧ p
-
-def Satisfiable (T : Theory L μ) : Prop :=
-  ∃ (M : Type u) (_ : Inhabited M) (s : Structure₁ L M), s ⊧ T
+end
 
 namespace SubFormula
 variable {L₁ L₂ : Language.{u}} {Φ : L₁ →ᵥ L₂} 
 
 section 
-variable {M : Type w} {s₂ : Structure₁ L₂ M} {n} {e : Fin n → M} {ε : μ → M}
+variable {M : Type u} {s₂ : Structure₁ L₂ M} {n} {e : Fin n → M} {ε : μ → M}
 
-lemma subVal_onSubFormula₁ {p : SubFormula L₁ μ n} :
-    SubVal s₂ e ε (Φ.onSubFormula₁ p) ↔ SubVal (Φ.onStructure₁ s₂) e ε p :=
+lemma eval_onSubFormula₁ {p : SubFormula L₁ μ n} :
+    Eval s₂ e ε (Φ.onSubFormula₁ p) ↔ Eval (Φ.onStructure₁ s₂) e ε p :=
   by induction p using rec' <;>
     simp[*, SubTerm.val_onSubTerm, Language.Hom.onSubFormula₁_rel, Language.Hom.onSubFormula₁_nrel,
-      subVal_rel, subVal_nrel]
+      eval_rel, eval_nrel]
 
-lemma models_onSubFormula₁ {p : Formula L₁ μ} :
-    s₂ ⊧ Φ.onSubFormula₁ p ↔ Φ.onStructure₁ s₂ ⊧ p :=
-  by simp[models_def, Val, subVal_onSubFormula₁]
+lemma models_onSubFormula₁ {σ : Sentence L₁} :
+    (toStruc s₂) ⊧ₛ (Φ.onSubFormula₁ σ) ↔ (toStruc $ Φ.onStructure₁ s₂) ⊧ₛ σ :=
+  by simp[modelsₛ_iff, Realize, eval_onSubFormula₁]
 
-lemma onSubFormula₁_models_onSubFormula₁ {T : Theory L₁ μ} {p : Formula L₁ μ} (h : T ⊧ p) :
-    Φ.onSubFormula₁ '' T ⊧ Φ.onSubFormula₁ p := by
-  intros M _ s hM
-  have : Φ.onStructure₁ s ⊧ p := h (Φ.onStructure₁ s) (fun q hq => models_onSubFormula₁.mp $ hM _ (Set.mem_image_of_mem _ hq))
+lemma onSubFormula₁_models_onSubFormula₁ {T : CTheory L₁} {σ : Sentence L₁} (h : T ⊨ σ) :
+    Φ.onSubFormula₁ '' T ⊨ Φ.onSubFormula₁ σ := by
+  simp[consequence_iff]
+  intro M _ s hM
+  have : (toStruc $ Φ.onStructure₁ s) ⊧ₛ σ :=
+    consequence_iff.mp h M (Φ.onStructure₁ s) (fun q hq => models_onSubFormula₁.mp $ hM (Set.mem_image_of_mem _ hq))
   exact models_onSubFormula₁.mpr this
 
 end
@@ -179,29 +171,31 @@ section
 variable
   (injf : ∀ k, Function.Injective (Φ.onFunc : L₁.func k → L₂.func k))
   (injr : ∀ k, Function.Injective (Φ.onRel : L₁.rel k → L₂.rel k))
-  {M : Type w} [Inhabited M] (s₁ : Structure₁ L₁ M)
+  {M : Type u} [Inhabited M] (s₁ : Structure₁ L₁ M)
   {n} (e : Fin n → M) (ε : μ → M)
 
-lemma subVal_extendStructure₁_onSubFormula₁ {p : SubFormula L₁ μ n} :
-    SubVal (Φ.extendStructure₁ s₁) e ε (Φ.onSubFormula₁ p) ↔ SubVal s₁ e ε p := by
+lemma eval_extendStructure₁_onSubFormula₁ {p : SubFormula L₁ μ n} :
+    Eval (Φ.extendStructure₁ s₁) e ε (Φ.onSubFormula₁ p) ↔ Eval s₁ e ε p := by
   induction p using rec' <;> simp[*, SubTerm.val_extendStructure₁_onSubTerm Φ e ε injf s₁,
-    Language.Hom.onSubFormula₁_rel, Language.Hom.onSubFormula₁_nrel, subVal_rel, subVal_nrel]
+    Language.Hom.onSubFormula₁_rel, Language.Hom.onSubFormula₁_nrel, eval_rel, eval_nrel]
   · case hrel k r v =>
     exact Structure₁.extendStructure₁_rel Φ s₁ (injr k) r (fun i => SubTerm.val s₁ e ε (v i))
   · case hnrel k r v =>
     simpa[not_iff_not] using
       Structure₁.extendStructure₁_rel Φ s₁ (injr k) r (fun i => SubTerm.val s₁ e ε (v i))
 
-lemma models_extendStructure₁_onSubFormula₁ {p : Formula L₁ μ} :
-    Φ.extendStructure₁ s₁ ⊧ Φ.onSubFormula₁ p ↔ s₁ ⊧ p := by
-  simp[models_def, Val, subVal_extendStructure₁_onSubFormula₁ injf injr]
+lemma models_extendStructure₁_onSubFormula₁ (σ : Sentence L₁) :
+    (toStruc $ Φ.extendStructure₁ s₁) ⊧ₛ (Φ.onSubFormula₁ σ) ↔ (toStruc s₁) ⊧ₛ σ := by
+  simp[modelsₛ_def, Realize, eval_extendStructure₁_onSubFormula₁ injf injr]
 
-lemma onSubFormula₁_models_onSubFormula₁_iff {T : Theory L₁ μ} {p : Formula L₁ μ} :
-    Φ.onSubFormula₁ '' T ⊧ Φ.onSubFormula₁ p ↔ T ⊧ p :=
-  ⟨by intros h M _ s₁ hs₁
-      exact (models_extendStructure₁_onSubFormula₁ injf injr s₁).mp $
-        h (Φ.extendStructure₁ s₁) (by simpa[models_extendStructure₁_onSubFormula₁ injf injr] using hs₁),
-   onSubFormula₁_models_onSubFormula₁⟩
+lemma onSubFormula₁_models_onSubFormula₁_iff {T : CTheory L₁} {σ : Sentence L₁} :
+    Φ.onSubFormula₁ '' T ⊨ Φ.onSubFormula₁ σ ↔ T ⊨ σ := by
+  constructor
+  · simp[consequence_iff, modelsTheory_def, models_iff_modelsₛ]; intro h M _ s₁ hs₁
+    exact (models_extendStructure₁_onSubFormula₁ injf injr s₁ σ).mp $
+      h M (Φ.extendStructure₁ s₁)
+        (fun σ hσ => (models_extendStructure₁_onSubFormula₁ injf injr s₁ σ).mpr (hs₁ hσ))
+  · exact onSubFormula₁_models_onSubFormula₁
 
 end
 
@@ -211,8 +205,8 @@ open Language
 variable {L : Language.{u}} [L.HasEq] {μ : Type v} (M : Type w) (s : Structure₁ L M) [Structure₁.Eq L M]
   {n} (e : Fin n → M) (ε : μ → M)
 
-@[simp] lemma subVal_eq (t u : SubTerm L μ n) :
-    SubVal s e ε (rel Language.HasEq.eq ![t, u]) ↔ t.val s e ε = u.val s e ε :=
+@[simp] lemma eval_eq (t u : SubTerm L μ n) :
+    Eval s e ε (rel Language.HasEq.eq ![t, u]) ↔ t.val s e ε = u.val s e ε :=
   by simp
 
 end Eq
